theories/heap_lang/lang.v
@@ -108,7 +108,7 @@ Inductive expr :=
   | NewProph
   | Resolve (e0 : expr) (e1 : expr) (e2 : expr) (* wrapped expr, proph, val *)
   (* trace stuff *)
-  | Emit (e1 : expr) (e2 : expr) (* tag, value *)
+  | Emit (e : expr)
   | Fresh (e : expr)
 with val :=
   | LitV (l : base_lit)
@@ -188,11 +188,10 @@ Definition vals_compare_safe (vl v1 : val) : Prop :=
   val_is_unboxed vl ∨ val_is_unboxed v1.
 Arguments vals_compare_safe !_ !_ /.
 
-Definition event : Type := (string * val).
 (** The state: heaps of vals. *)
 Record state : Type := {
   heap: gmap loc val;
-  trace: list event;
+  trace: list val;
   used_proph_id: gset proph_id;
 }.
 
@@ -248,7 +247,7 @@ Proof.
      | NewProph, NewProph => left _
      | Resolve e0 e1 e2, Resolve e0' e1' e2' =>
         cast_if_and3 (decide (e0 = e0')) (decide (e1 = e1')) (decide (e2 = e2'))
-     | Emit s1 e1, Emit s2 e2 => cast_if_and (decide (s1 = s2)) (decide (e1 = e2))
+     | Emit e1, Emit e2 => cast_if (decide (e1 = e2))
      | Fresh e1, Fresh e2 => cast_if (decide (e1 = e2))
      | _, _ => right _
      end
@@ -331,7 +330,7 @@ Proof.
      | FAA e1 e2 => GenNode 17 [go e1; go e2]
      | NewProph => GenNode 18 []
      | Resolve e0 e1 e2 => GenNode 19 [go e0; go e1; go e2]
-     | Emit e1 e2 => GenNode 20 [go e1; go e2]
+     | Emit e => GenNode 20 [go e]
      | Fresh e => GenNode 21 [go e]
     end
    with gov v :=
@@ -368,7 +367,7 @@ Proof.
      | GenNode 17 [e1; e2] => FAA (go e1) (go e2)
      | GenNode 18 [] => NewProph
      | GenNode 19 [e0; e1; e2] => Resolve (go e0) (go e1) (go e2)
-     | GenNode 20 [e1; e2] => Emit (go e1) (go e2)
+     | GenNode 20 [e] => Emit (go e)
      | GenNode 21 [e] => Fresh (go e)
      | _ => Val $ LitV LitUnit (* dummy *)
      end
@@ -429,8 +428,7 @@ Inductive ectx_item :=
   | ResolveLCtx (ctx : ectx_item) (v1 : val) (v2 : val)
   | ResolveMCtx (e0 : expr) (v2 : val)
   | ResolveRCtx (e0 : expr) (e1 : expr)
-  | EmitLCtx (v2 : val)
-  | EmitRCtx (e1 : expr)
+  | EmitCtx
   | FreshCtx.
 
 (** Contextual closure will only reduce [e] in [Resolve e (Val _) (Val _)] if
@@ -468,8 +466,7 @@ Fixpoint fill_item (Ki : ectx_item) (e : expr) : expr :=
   | ResolveLCtx K v1 v2 => Resolve (fill_item K e) (Val v1) (Val v2)
   | ResolveMCtx ex v2 => Resolve ex e (Val v2)
   | ResolveRCtx ex e1 => Resolve ex e1 e
-  | EmitLCtx v2 => Emit e (of_val v2)
-  | EmitRCtx e1 => Emit e1 e
+  | EmitCtx => Emit e
   | FreshCtx => Fresh e
   end.
 
@@ -498,7 +495,7 @@ Fixpoint subst (x : string) (v : val) (e : expr)  : expr :=
   | FAA e1 e2 => FAA (subst x v e1) (subst x v e2)
   | NewProph => NewProph
   | Resolve ex e1 e2 => Resolve (subst x v ex) (subst x v e1) (subst x v e2)
-  | Emit e1 e2 => Emit (subst x v e1) (subst x v e2)
+  | Emit e => Emit (subst x v e)
   | Fresh e => Fresh (subst x v e)
   end.
 
@@ -569,8 +566,8 @@ Definition state_upd_heap (f: gmap loc val → gmap loc val) (σ: state) : state
   {| heap := f σ.(heap); trace := σ.(trace); used_proph_id := σ.(used_proph_id) |}.
 Arguments state_upd_heap _ !_ /.
 
-Definition state_add_event (e: event) (σ: state) : state :=
-  {| heap := σ.(heap); trace := σ.(trace) ++ [e]; used_proph_id := σ.(used_proph_id) |}.
+Definition state_add_event (v: val) (σ: state) : state :=
+  {| heap := σ.(heap); trace := σ.(trace) ++ [v]; used_proph_id := σ.(used_proph_id) |}.
 Arguments state_add_event _ !_ /.
 
 Definition state_upd_used_proph_id (f: gset proph_id → gset proph_id) (σ: state) : state :=
@@ -627,8 +624,8 @@ Proof.
   rewrite right_id insert_union_singleton_l. done.
 Qed.
 
-Definition fresh_tag (tag: string) (t: list event) :=
-  ∀ v, (tag, v) ∉ t.
+Definition fresh_tag (tag: string) (t: list val) :=
+  ∀ (v: val), (PairV (LitV (LitTag tag)) v) ∉ t.
 
 Inductive head_step : expr → state → list observation → expr → state → list expr → Prop :=
   | RecS f x e σ :
@@ -703,14 +700,14 @@ Inductive head_step : expr → state → list observation → expr → state →
      head_step e σ κs (Val v) σ' ts →
      head_step (Resolve e (Val $ LitV $ LitProphecy p) (Val w)) σ
                (κs ++ [(p, (v, w))]) (Val v) σ' ts
-  | EmitS tag v σ :
-     head_step (Emit (Val $ LitV (LitTag tag)) (Val v)) σ [] (Val $ LitV LitUnit)
-               (state_add_event (tag, v) σ) []
+  | EmitS v σ :
+     head_step (Emit (Val v)) σ [] (Val $ LitV LitUnit)
+               (state_add_event v σ) []
 
   | FreshS v σ tag :
     fresh_tag tag σ.(trace) →
     head_step (Fresh (Val v)) σ [] (Val $ LitV (LitTag tag))
-              (state_add_event (tag, v) σ) [].
+              (state_add_event (PairV (LitV (LitTag tag)) v) σ) [].
 
 (** Basic properties about the language *)
 Instance fill_item_inj Ki : Inj (=) (=) (fill_item Ki).
