theories/iterator.v
@@ -5,7 +5,7 @@ From intensional.heap_lang Require Import lifting proofmode notation.
 From intensional.heap_lang Require Import adequacy.
 From intensional Require Import stdpp_extra tactics.
 Set Default Proof Using "Type".
-Implicit Types t : list event.
+Implicit Types t : list val.
 
 Definition size_spec `{!heapG Σ} (Coll: val → iProp Σ) (Iter: val → val → iProp Σ) (size: val): iProp Σ :=
   ∀ c, {{{ Coll c }}} size #() {{{ x, RET x; Coll c }}}.
@@ -38,10 +38,10 @@ Definition iterlib_spec `{!heapG Σ} (P0: iProp Σ) (lib: val): iProp Σ :=
 Section Trace.
 
 Definition iterator_trace t :=
-  ∀ (i:nat) l, t !! i = Some ("next", l) →
-    ∃ (j:nat), j < i ∧ t !! j = Some ("iterator", l) ∧
-               ∀ (k:nat), j < k < i → t !! k ≠ Some ("add", #()) ∧
-                                      t !! k ≠ Some ("remove", #()).
+  ∀ (i:nat) l, t !! i = Some (#"next", l)%V →
+    ∃ (j:nat), j < i ∧ t !! j = Some (#"iterator", l)%V ∧
+               ∀ (k:nat), j < k < i → t !! k ≠ Some (#"add", #())%V ∧
+                                      t !! k ≠ Some (#"remove", #())%V.
 
 Lemma iterator_trace_nil :
   iterator_trace [].
@@ -49,32 +49,32 @@ Proof. unfold iterator_trace. go*. Qed.
 
 Lemma iterator_trace_size t :
   iterator_trace t →
-  iterator_trace (t ++ [("size", #())]).
+  iterator_trace (t ++ [(#"size", #())%V]).
 Proof. unfold iterator_trace. go*. Qed.
 
 Lemma iterator_trace_add t :
   iterator_trace t →
-  iterator_trace (t ++ [("add", #())]).
+  iterator_trace (t ++ [(#"add", #())%V]).
 Proof. unfold iterator_trace. go*. Qed.
 
 Lemma iterator_trace_remove t :
   iterator_trace t →
-  iterator_trace (t ++ [("remove", #())]).
+  iterator_trace (t ++ [(#"remove", #())%V]).
 Proof. unfold iterator_trace. go*. Qed.
 
 Lemma iterator_trace_iterator t x :
   iterator_trace t →
-  iterator_trace (t ++ [("iterator", x)]).
+  iterator_trace (t ++ [(#"iterator", x)%V]).
 Proof. unfold iterator_trace. go*. Qed.
 
 Lemma iterator_trace_next t t' (n0 k: nat) x :
-  t' !! k = Some ("iterator", x) →
+  t' !! k = Some (#"iterator", x)%V →
   t' `prefix_of` t →
   n0 ≤ k →
-  (∀ (k:nat) lbl,
-     n0 ≤ k → t !! k = Some (lbl, #()) → lbl ≠ "add" ∧ lbl ≠ "remove") →
+  (∀ (k:nat) (tag:string),
+     n0 ≤ k → t !! k = Some (#tag, #())%V → tag ≠ "add" ∧ tag ≠ "remove") →
   iterator_trace t →
-  iterator_trace (t ++ [("next", x)]).
+  iterator_trace (t ++ [(#"next", x)%V]).
 Proof. unfold iterator_trace. go*. Qed.
 
 End Trace.
@@ -90,30 +90,30 @@ Context (Coll_impl: val → iProp Σ) (Iter_impl: val → val → iProp Σ).
 Context (size_impl add_impl remove_impl iterator_impl next_impl: val).
 
 Definition size : val :=
-  λ: "_", let: "r" := size_impl #() in Emit #"size" #() ;; "r".
+  λ: "_", let: "r" := size_impl #() in Emit (#"size", #()) ;; "r".
 
 Definition add : val :=
-  λ: "x", add_impl "x" ;; Emit #"add" #().
+  λ: "x", add_impl "x" ;; Emit (#"add", #()).
 
 Definition remove : val :=
-  λ: "x", remove_impl "x" ;; Emit #"remove" #().
+  λ: "x", remove_impl "x" ;; Emit (#"remove", #()).
 
 Definition iterator : val :=
-  λ: "_", let: "r" := iterator_impl #() in Emit #"iterator" "r" ;; "r".
+  λ: "_", let: "r" := iterator_impl #() in Emit (#"iterator", "r") ;; "r".
 
 Definition next : val :=
-  λ: "x", let: "r" := next_impl "x" in Emit #"next" "x" ;; "r".
+  λ: "x", let: "r" := next_impl "x" in Emit (#"next", "x") ;; "r".
 
 Definition Coll (x: val) : iProp Σ :=
   ∃ (y:val) (n: nat), ⌜x = (y, # n)%V⌝ ∗ Coll_impl y ∗
   ∃ t, trace_is t ∗ trace_inv N iterator_trace ∗
        ⌜n ≤ length t⌝ ∗
-       ⌜∀ (k:nat) lbl, n ≤ k → t !! k = Some (lbl, #()) →
-                       lbl ≠ "add" ∧ lbl ≠ "remove"⌝.
+       ⌜∀ (k:nat) (tag:string), n ≤ k → t !! k = Some (#tag, #())%V →
+                                tag ≠ "add" ∧ tag ≠ "remove"⌝.
 
 Definition Iter (r x: val) : iProp Σ :=
   ∃ (y:val) (n: nat), ⌜x = (y, # n)%V⌝ ∗ Iter_impl r y ∗
-  ∃ t, hist t ∗ ⌜∃ (k:nat), n ≤ k ∧ t !! k = Some ("iterator", r)⌝.
+  ∃ t, hist t ∗ ⌜∃ (k:nat), n ≤ k ∧ t !! k = Some (#"iterator", r)%V⌝.
 
 Lemma size_correct :
   size_spec Coll_impl Iter_impl size_impl -∗
@@ -124,7 +124,7 @@ Proof.
   iDestruct "Hc" as (? ? ?) "(? & Ht)". iDestruct "Ht" as (t) "(Ht & #HI & %)".
   iMod (trace_is_inv with "Ht HI") as "(Ht & %)".
   iApply ("spec" with "[$]"). iIntros "!>" (?) "Hc". wp_pures.
-  wp_bind (Emit _ _). iApply (wp_emit with "[$Ht $HI]"); eauto.
+  wp_bind (Emit _). iApply (wp_emit with "[$Ht $HI]"); eauto.
   by apply iterator_trace_size.
   iIntros "!> Ht". wp_pures. iApply "Hφ". unfold Coll.
   iExists _, _. iFrame. iSplitR; eauto. iExists _. iFrame "HI ∗". iPureIntro. go*.
@@ -169,7 +169,7 @@ Proof.
   iDestruct "Hc" as (? ? ?) "(? & Ht)". iDestruct "Ht" as (t) "(Ht & #HI & [% %])".
   iMod (trace_is_inv with "Ht HI") as "(Ht & %)".
   iApply ("spec" with "[$]"). iIntros "!>" (?) "(Hc & Hi)". wp_pures.
-  wp_bind (Emit _ _). iApply (wp_emit with "[$Ht $HI]"); eauto.
+  wp_bind (Emit _). iApply (wp_emit with "[$Ht $HI]"); eauto.
   by apply iterator_trace_iterator.
   iIntros "!> Ht". wp_pures.
   iDestruct (alloc_hist with "Ht") as "(Ht & Hh)".
@@ -193,7 +193,7 @@ Proof.
   iDestruct (hist_trace_is_prefix with "Ht Ht'") as %?.
   iMod (trace_is_inv with "Ht HI") as "(Ht & %)".
   iApply ("spec" with "[$]"). iIntros "!> (Hc & Hi)". wp_pures.
-  wp_bind (Emit _ _). iApply (wp_emit with "[$Ht $HI]"); eauto.
+  wp_bind (Emit _). iApply (wp_emit with "[$Ht $HI]"); eauto.
   { go. by eapply iterator_trace_next. }
   iIntros "!> Ht". wp_pures.
   iDestruct (alloc_hist with "Ht") as "(Ht & Hh)".
